Better implementation of ifc in DM

examples/dm4free/ifc.fst
@@ -7,22 +7,26 @@ type label =
   | Low
   | High
 
-let join l1 l2 = match l1, l2 with 
-  | _, High
-  | High, _ -> High
-  | _ -> Low
+let join l1 l2 =
+  match l1, l2 with
+  | _   , High
+  | High, _    -> High
+  | _   , _    -> Low
+
+let flows l1 l2 =
+  match l1, l2 with
+  | High, Low -> false
+  | _   , _   -> true
 
 type err (a:Type) =
   | Leak 
   | Result : v:a -> err a
-open FStar.FunctionalExtensionality
 
-let ifc (a:Type) = l0:label  //sensitivity of data seen so far, analogous to the PC label
-		 -> Tot (err (a 
-			     * l1:label{join l0 l1 = l1} //sensitivity of data computed by this computation, at least as much as what was seen so far; Need this invariant to prove the monad laws
-			     )
-		       )
-let eq_ifc (a:Type) (f:ifc a) (g:ifc a) = 
+let ifc (a:Type) = label -> Tot (err (a * label))
+
+(* open FStar.FunctionalExtensionality *)
+
+let eq_ifc (a:Type) (f:ifc a) (g:ifc a) =
    forall l. f l == g l
 
 let return_ifc (a:Type) (x:a) : ifc a = fun l -> Result (x, l)
@@ -32,7 +36,7 @@ let bind_ifc (a:Type) (b:Type) (f:ifc a) (g: a -> Tot (ifc b)) : ifc b
 	   | Result (x, l1) -> 
 	     match g x l1 with
 	     | Leak -> Leak
-	     | Result (y, l2) -> Result(y, join l1 l2)
+	     | Result (y, l2) -> Result(y, l2)
 
 val left_unit: a:Type -> b:Type -> x:a -> f:(a -> Tot (ifc b)) 
 	    -> Lemma (eq_ifc b (bind_ifc a b (return_ifc a x) f) (f x))
@@ -45,13 +49,23 @@ val associativity: a:Type -> b:Type -> c:Type -> f:ifc a -> g:(a -> Tot (ifc b))
 		 -> Lemma (eq_ifc c (bind_ifc a c f (fun x -> bind_ifc b c (g x) h)) (bind_ifc b c (bind_ifc a b f g) h))
 let associativity a b c f g h = ()		 
 
-//Some dummy implementations of actions for illustration purposes
-//Probably better to just take them axiomatically
-let read_low () : ifc nat = fun l -> Result (0, l)
-let read_high () : ifc nat = fun l -> Result (42, High)
-let write_low () : ifc unit = fun l -> 
-  match l with 
-  | High -> Leak
-  | _ -> Result((), l)
-let write_high () : ifc unit = fun l -> Result ((), l)
-  
+// Some dummy implementations of actions for illustration purposes
+// Probably better to just take them axiomatically
+let read (l:label) : ifc bool = fun l0 -> Result (true, join l0 l)
+let write (l:label) (b:bool) : ifc unit =
+  fun l0 -> if flows l0 l then (Result ((), l0)) else Leak
+
+let xor (b1:bool) (b2:bool) : Tot bool = not (b1 = b2)
+
+// A sample monadic program (normally would write this after
+// elaboration, but whatever, can write this in DM too)
+val p : unit -> Pure (ifc unit) (requires True) (ensures (fun r -> forall l. r l = Leak))
+(* Weak type (works): unit -> Tot (ifc unit) *)
+(* Alternative strong type (doesn't work), (Valid(ApplyTT@2 @0))
+  unit -> Tot (label -> Pure (err (unit * label)) (requires True) (ensures (fun r -> r = Leak))) *)
+let p () = bind_ifc _ _ (read Low)              (fun b1 ->
+           bind_ifc _ _ (read Low)              (fun b2 ->
+           bind_ifc _ _ (write Low (b1 && b2))  (fun _  ->
+           bind_ifc _ _ (read High)             (fun b3 ->
+           bind_ifc _ _ (write High (b1 || b3)) (fun _  ->
+                        (write Low (xor b3 b3))  )))))
